lib/Base/NativeArrays.s.dfy
@@ -1,24 +1,42 @@
 include "NativeTypes.s.dfy"
 
-module {:extern} TotalOrderNative {
+module {:extern} NativeArrays {
   import opened NativeTypes
 
-  class Arrays
+  predicate lt(a: seq<byte>, b: seq<byte>)
   {
-    static predicate lt(a: seq<byte>, b: seq<byte>)
-    {
-      if |a| == 0 && |b| == 0 then false
-      else if |a| == 0 then true
-      else if |b| == 0 then false
-      else if a[0] < b[0] then true
-      else if a[0] > b[0] then false
-      else lt(a[1..], b[1..])
-    }
-
-    static method{:axiom} ByteSeqCmpByteSeq(s1: seq<byte>, s2: seq<byte>)
-        returns (c : int32)
-        ensures c < 0 ==> lt(s1, s2)
-        ensures c > 0 ==> lt(s2, s1)
-        ensures c == 0 ==> s1 == s2
+    if |a| == 0 && |b| == 0 then false
+    else if |a| == 0 then true
+    else if |b| == 0 then false
+    else if a[0] < b[0] then true
+    else if a[0] > b[0] then false
+    else lt(a[1..], b[1..])
   }
+
+  method {:axiom} ByteSeqCmpByteSeq(s1: seq<byte>, s2: seq<byte>)
+      returns (c : int32)
+      ensures c < 0 ==> lt(s1, s2)
+      ensures c > 0 ==> lt(s2, s1)
+      ensures c == 0 ==> s1 == s2
+
+  method {:axiom} newArrayFill<T>(n: uint64, t: T) returns (ar: array<T>)
+  ensures ar.Length == n as int
+  ensures forall i | 0 <= i < n :: ar[i] == t
+  ensures fresh(ar)
+
+  method {:axiom} newArrayClone<T>(ar: array<T>) returns (ar': array<T>)
+  ensures ar[..] == ar'[..]
+  ensures fresh(ar')
+
+  method {:axiom} CopySeqIntoArray<A>(src:seq<A>, srcIndex:uint64, dst:array<A>, dstIndex:uint64, len:uint64)
+      requires (srcIndex) as int + (len as int) <= |src|;
+      requires (dstIndex as int) + (len as int) <= dst.Length;
+      modifies dst;
+      ensures  forall i :: 0 <= i < dst.Length ==> dst[i] == (
+                  if (dstIndex as int) <= i < (dstIndex as int) + (len as int)
+                  then src[i - (dstIndex as int) + (srcIndex as int)]
+                  else old(dst[..])[i]);
+      ensures  forall i :: (srcIndex as int) <= i < (srcIndex as int) + (len as int) ==>
+                  src[i] == dst[i - (srcIndex as int) + (dstIndex as int)];
+
 }
