lib/Base/NativeBenchmarking.s.dfy
@@ -1,0 +1,4 @@
+module {:extern} NativeBenchmarking {
+  method {:axiom} start()
+  method {:axiom} end()
+}
